\documentclass{article}%
\usepackage[T1]{fontenc}%
\usepackage[utf8]{inputenc}%
\usepackage{lmodern}%
\usepackage{textcomp}%
\usepackage{lastpage}%
\usepackage[margin=0.5in]{geometry}%
\usepackage{ragged2e}%
%
\title{Distributivité}%
\author{Niveau de difficulté : debutant}%
\date{{}}%
%
\begin{document}%
\normalsize%
\pagestyle{empty}%
\maketitle%
\section{Enoncé}%
\label{sec:Enonc}%
Développer et réduire les expressions suivantes :%
\newline%
%
\newline%
%
\begin{minipage}{0.5\textwidth}%
A=$(1+24t)(-27+8t)$\\%
\end{minipage}%
\begin{minipage}{0.5\textwidth}%
B=$(11-15z)(31z+6)$\\%
\end{minipage}%
\\%
\begin{minipage}{0.5\textwidth}%
C=$(3x-44)(-36-47x)$\\%
\end{minipage}%
\begin{minipage}{0.5\textwidth}%
D=$(49z-32)(-38+16z)$\\%
\end{minipage}%
\\%
\begin{minipage}{0.5\textwidth}%
E=$(-19z-4)(12z-20)$\\%
\end{minipage}%
\begin{minipage}{0.5\textwidth}%
F=$(-37y-24)(-19+36y)$\\%
\end{minipage}%
\\%
\begin{minipage}{0.5\textwidth}%
G=$(22+12x)(-48x+28)$\\%
\end{minipage}%
\begin{minipage}{0.5\textwidth}%
H=$(28z-7)(8z+18)$\\%
\end{minipage}%
\\%
\begin{minipage}{0.5\textwidth}%
I=$(-25y-26)(-23+49y)$\\%
\end{minipage}%
\begin{minipage}{0.5\textwidth}%
J=$(-46-16y)(8+30y)$\\%
\end{minipage}%
\\

%
\newpage%
\section{Corrigé}%
\label{sec:Corrig}%
\begin{minipage}{0.5\textwidth}%
A=$(1+24t)(-27+8t)$\\%
A=$1 \times (-27)+1 \times 8t+24t \times (-27)+24t \times 8t$\\%
A=$-27+8t-648t+192t^2$\\%
A=$192t^2+8t-648t-27$\\%
A=$192t^2-640t-27$\\%
\end{minipage}%
\begin{minipage}{0.5\textwidth}%
B=$(11-15z)(31z+6)$\\%
B=$11 \times 31z+11 \times 6-15z \times 31z-15z \times 6$\\%
B=$341z+66-465z^2-90z$\\%
B=$-465z^2+341z-90z+66$\\%
B=$-465z^2+251z+66$\\%
\end{minipage}%
\\%
\begin{minipage}{0.5\textwidth}%
C=$(3x-44)(-36-47x)$\\%
C=$3x \times (-36)+3x \times (-47x)-44 \times (-36)-44 \times (-47x)$\\%
C=$-108x-141x^2+1584+2068x$\\%
C=$-141x^2-108x+2068x+1584$\\%
C=$-141x^2+1960x+1584$\\%
\end{minipage}%
\begin{minipage}{0.5\textwidth}%
D=$(49z-32)(-38+16z)$\\%
D=$49z \times (-38)+49z \times 16z-32 \times (-38)-32 \times 16z$\\%
D=$-1862z+784z^2+1216-512z$\\%
D=$784z^2-1862z-512z+1216$\\%
D=$784z^2-2374z+1216$\\%
\end{minipage}%
\\%
\begin{minipage}{0.5\textwidth}%
E=$(-19z-4)(12z-20)$\\%
E=$-19z \times 12z-19z \times (-20)-4 \times 12z-4 \times (-20)$\\%
E=$-228z^2+380z-48z+80$\\%
E=$-228z^2+332z+80$\\%
\end{minipage}%
\begin{minipage}{0.5\textwidth}%
F=$(-37y-24)(-19+36y)$\\%
F=$-37y \times (-19)-37y \times 36y-24 \times (-19)-24 \times 36y$\\%
F=$703y-1332y^2+456-864y$\\%
F=$-1332y^2+703y-864y+456$\\%
F=$-1332y^2-161y+456$\\%
\end{minipage}%
\\%
\begin{minipage}{0.5\textwidth}%
G=$(22+12x)(-48x+28)$\\%
G=$22 \times (-48x)+22 \times 28+12x \times (-48x)+12x \times 28$\\%
G=$-1056x+616-576x^2+336x$\\%
G=$-576x^2-1056x+336x+616$\\%
G=$-576x^2-720x+616$\\%
\end{minipage}%
\begin{minipage}{0.5\textwidth}%
H=$(28z-7)(8z+18)$\\%
H=$28z \times 8z+28z \times 18-7 \times 8z-7 \times 18$\\%
H=$224z^2+504z-56z-126$\\%
H=$224z^2+448z-126$\\%
\end{minipage}%
\\%
\begin{minipage}{0.5\textwidth}%
I=$(-25y-26)(-23+49y)$\\%
I=$-25y \times (-23)-25y \times 49y-26 \times (-23)-26 \times 49y$\\%
I=$575y-1225y^2+598-1274y$\\%
I=$-1225y^2+575y-1274y+598$\\%
I=$-1225y^2-699y+598$\\%
\end{minipage}%
\begin{minipage}{0.5\textwidth}%
J=$(-46-16y)(8+30y)$\\%
J=$-46 \times 8-46 \times 30y-16y \times 8-16y \times 30y$\\%
J=$-368-1380y-128y-480y^2$\\%
J=$-480y^2-1380y-128y-368$\\%
J=$-480y^2-1508y-368$\\%
\end{minipage}%
\\

%
\end{document}