\documentclass{article}%
\usepackage[T1]{fontenc}%
\usepackage[utf8]{inputenc}%
\usepackage{lmodern}%
\usepackage{textcomp}%
\usepackage{lastpage}%
\usepackage[margin=0.5in]{geometry}%
\usepackage{ragged2e}%
%
\title{Distributivité}%
\author{Niveau de difficulté : intermédiaire ++}%
\date{{}}%
%
\begin{document}%
\normalsize%
\pagestyle{empty}%
\maketitle%
\section{Enoncé}%
\label{sec:Enonc}%
Développer et réduire les expressions suivantes :%
\newline%
%
\newline%
%
\begin{minipage}{0.5\textwidth}%
A=$(-27t+28)(43t-30)$\\%
\end{minipage}%
\begin{minipage}{0.5\textwidth}%
B=$(-48x+30)(-42x+23)$\\%
\end{minipage}%
\\%
\begin{minipage}{0.5\textwidth}%
C=$(38+36z)(-26+10z)$\\%
\end{minipage}%
\begin{minipage}{0.5\textwidth}%
D=$(-19z-1)(18-3z)$\\%
\end{minipage}%
\\%
\begin{minipage}{0.5\textwidth}%
E=$(-13-8t)(-50t+34)$\\%
\end{minipage}%
\begin{minipage}{0.5\textwidth}%
F=$(-16t+23)(28-46t)$\\%
\end{minipage}%
\\%
\begin{minipage}{0.5\textwidth}%
G=$(-32-4t)(-15-24t)$\\%
\end{minipage}%
\begin{minipage}{0.5\textwidth}%
H=$(-16-38x)(-35x-33)$\\%
\end{minipage}%
\\%
\begin{minipage}{0.5\textwidth}%
I=$(-5+32x)(49x-27)$\\%
\end{minipage}%
\begin{minipage}{0.5\textwidth}%
J=$(16t-36)(8t+37)$\\%
\end{minipage}%
\\%
\begin{minipage}{0.5\textwidth}%
K=$(5x+24)(13+15x)$\\%
\end{minipage}%
\begin{minipage}{0.5\textwidth}%
L=$(30x+7)(21x-19)$\\%
\end{minipage}%
\\%
\begin{minipage}{0.5\textwidth}%
M=$(-29-5z)(-35-33z)$\\%
\end{minipage}%
\begin{minipage}{0.5\textwidth}%
N=$(-30-36t)(27t+6)$\\%
\end{minipage}%
\\%
\begin{minipage}{0.5\textwidth}%
O=$(-24x-33)(23-6x)$\\%
\end{minipage}%
\begin{minipage}{0.5\textwidth}%
P=$(-50z-33)(-25z+40)$\\%
\end{minipage}%
\\%
\begin{minipage}{0.5\textwidth}%
Q=$(-36z-28)(18-25z)$\\%
\end{minipage}%
\begin{minipage}{0.5\textwidth}%
R=$(8t-42)(-4-45t)$\\%
\end{minipage}%
\\%
\begin{minipage}{0.5\textwidth}%
S=$(-41+9x)(-10x-19)$\\%
\end{minipage}%
\begin{minipage}{0.5\textwidth}%
T=$(-23+21z)(-6z-27)$\\%
\end{minipage}%
\\

%
\newpage%
\section{Corrigé}%
\label{sec:Corrig}%
\begin{minipage}{0.5\textwidth}%
A=$(-27t+28)(43t-30)$\\%
A=$-27t \times 43t-27t \times (-30)+28 \times 43t+28 \times (-30)$\\%
A=$-1161t^2+810t+1204t-840$\\%
A=$-1161t^2+2014t-840$\\%
\end{minipage}%
\begin{minipage}{0.5\textwidth}%
B=$(-48x+30)(-42x+23)$\\%
B=$-48x \times (-42x)-48x \times 23+30 \times (-42x)+30 \times 23$\\%
B=$2016x^2-1104x-1260x+690$\\%
B=$2016x^2-2364x+690$\\%
\end{minipage}%
\\%
\begin{minipage}{0.5\textwidth}%
C=$(38+36z)(-26+10z)$\\%
C=$38 \times (-26)+38 \times 10z+36z \times (-26)+36z \times 10z$\\%
C=$-988+380z-936z+360z^2$\\%
C=$360z^2+380z-936z-988$\\%
C=$360z^2-556z-988$\\%
\end{minipage}%
\begin{minipage}{0.5\textwidth}%
D=$(-19z-1)(18-3z)$\\%
D=$-19z \times 18-19z \times (-3z)-1 \times 18-1 \times (-3z)$\\%
D=$-342z+57z^2-18+3z$\\%
D=$57z^2-342z+3z-18$\\%
D=$57z^2-339z-18$\\%
\end{minipage}%
\\%
\begin{minipage}{0.5\textwidth}%
E=$(-13-8t)(-50t+34)$\\%
E=$-13 \times (-50t)-13 \times 34-8t \times (-50t)-8t \times 34$\\%
E=$650t-442+400t^2-272t$\\%
E=$400t^2+650t-272t-442$\\%
E=$400t^2+378t-442$\\%
\end{minipage}%
\begin{minipage}{0.5\textwidth}%
F=$(-16t+23)(28-46t)$\\%
F=$-16t \times 28-16t \times (-46t)+23 \times 28+23 \times (-46t)$\\%
F=$-448t+736t^2+644-1058t$\\%
F=$736t^2-448t-1058t+644$\\%
F=$736t^2-1506t+644$\\%
\end{minipage}%
\\%
\begin{minipage}{0.5\textwidth}%
G=$(-32-4t)(-15-24t)$\\%
G=$-32 \times (-15)-32 \times (-24t)-4t \times (-15)-4t \times (-24t)$\\%
G=$480+768t+60t+96t^2$\\%
G=$96t^2+768t+60t+480$\\%
G=$96t^2+828t+480$\\%
\end{minipage}%
\begin{minipage}{0.5\textwidth}%
H=$(-16-38x)(-35x-33)$\\%
H=$-16 \times (-35x)-16 \times (-33)-38x \times (-35x)-38x \times (-33)$\\%
H=$560x+528+1330x^2+1254x$\\%
H=$1330x^2+560x+1254x+528$\\%
H=$1330x^2+1814x+528$\\%
\end{minipage}%
\\%
\begin{minipage}{0.5\textwidth}%
I=$(-5+32x)(49x-27)$\\%
I=$-5 \times 49x-5 \times (-27)+32x \times 49x+32x \times (-27)$\\%
I=$-245x+135+1568x^2-864x$\\%
I=$1568x^2-245x-864x+135$\\%
I=$1568x^2-1109x+135$\\%
\end{minipage}%
\begin{minipage}{0.5\textwidth}%
J=$(16t-36)(8t+37)$\\%
J=$16t \times 8t+16t \times 37-36 \times 8t-36 \times 37$\\%
J=$128t^2+592t-288t-1332$\\%
J=$128t^2+304t-1332$\\%
\end{minipage}%
\\%
\begin{minipage}{0.5\textwidth}%
K=$(5x+24)(13+15x)$\\%
K=$5x \times 13+5x \times 15x+24 \times 13+24 \times 15x$\\%
K=$65x+75x^2+312+360x$\\%
K=$75x^2+65x+360x+312$\\%
K=$75x^2+425x+312$\\%
\end{minipage}%
\begin{minipage}{0.5\textwidth}%
L=$(30x+7)(21x-19)$\\%
L=$30x \times 21x+30x \times (-19)+7 \times 21x+7 \times (-19)$\\%
L=$630x^2-570x+147x-133$\\%
L=$630x^2-423x-133$\\%
\end{minipage}%
\\%
\begin{minipage}{0.5\textwidth}%
M=$(-29-5z)(-35-33z)$\\%
M=$-29 \times (-35)-29 \times (-33z)-5z \times (-35)-5z \times (-33z)$\\%
M=$1015+957z+175z+165z^2$\\%
M=$165z^2+957z+175z+1015$\\%
M=$165z^2+1132z+1015$\\%
\end{minipage}%
\begin{minipage}{0.5\textwidth}%
N=$(-30-36t)(27t+6)$\\%
N=$-30 \times 27t-30 \times 6-36t \times 27t-36t \times 6$\\%
N=$-810t-180-972t^2-216t$\\%
N=$-972t^2-810t-216t-180$\\%
N=$-972t^2-1026t-180$\\%
\end{minipage}%
\\%
\begin{minipage}{0.5\textwidth}%
O=$(-24x-33)(23-6x)$\\%
O=$-24x \times 23-24x \times (-6x)-33 \times 23-33 \times (-6x)$\\%
O=$-552x+144x^2-759+198x$\\%
O=$144x^2-552x+198x-759$\\%
O=$144x^2-354x-759$\\%
\end{minipage}%
\begin{minipage}{0.5\textwidth}%
P=$(-50z-33)(-25z+40)$\\%
P=$-50z \times (-25z)-50z \times 40-33 \times (-25z)-33 \times 40$\\%
P=$1250z^2-2000z+825z-1320$\\%
P=$1250z^2-1175z-1320$\\%
\end{minipage}%
\\%
\begin{minipage}{0.5\textwidth}%
Q=$(-36z-28)(18-25z)$\\%
Q=$-36z \times 18-36z \times (-25z)-28 \times 18-28 \times (-25z)$\\%
Q=$-648z+900z^2-504+700z$\\%
Q=$900z^2-648z+700z-504$\\%
Q=$900z^2+52z-504$\\%
\end{minipage}%
\begin{minipage}{0.5\textwidth}%
R=$(8t-42)(-4-45t)$\\%
R=$8t \times (-4)+8t \times (-45t)-42 \times (-4)-42 \times (-45t)$\\%
R=$-32t-360t^2+168+1890t$\\%
R=$-360t^2-32t+1890t+168$\\%
R=$-360t^2+1858t+168$\\%
\end{minipage}%
\\%
\begin{minipage}{0.5\textwidth}%
S=$(-41+9x)(-10x-19)$\\%
S=$-41 \times (-10x)-41 \times (-19)+9x \times (-10x)+9x \times (-19)$\\%
S=$410x+779-90x^2-171x$\\%
S=$-90x^2+410x-171x+779$\\%
S=$-90x^2+239x+779$\\%
\end{minipage}%
\begin{minipage}{0.5\textwidth}%
T=$(-23+21z)(-6z-27)$\\%
T=$-23 \times (-6z)-23 \times (-27)+21z \times (-6z)+21z \times (-27)$\\%
T=$138z+621-126z^2-567z$\\%
T=$-126z^2+138z-567z+621$\\%
T=$-126z^2-429z+621$\\%
\end{minipage}%
\\

%
\end{document}