\documentclass{article}%
\usepackage[T1]{fontenc}%
\usepackage[utf8]{inputenc}%
\usepackage{lmodern}%
\usepackage{textcomp}%
\usepackage{lastpage}%
\usepackage[margin=0.5in]{geometry}%
\usepackage{ragged2e}%
%
\title{Distributivité}%
\author{Niveau de difficulté : difficile}%
\date{{}}%
%
\begin{document}%
\normalsize%
\pagestyle{empty}%
\maketitle%
\section{Enoncé}%
\label{sec:Enonc}%
Développer et réduire les expressions suivantes :%
\newline%
%
\newline%
%
\begin{minipage}{0.5\textwidth}%
A=$(-4y+44)(47-50y)$\\%
\end{minipage}%
\begin{minipage}{0.5\textwidth}%
B=$(-23+t)(35t+9)$\\%
\end{minipage}%
\\%
\begin{minipage}{0.5\textwidth}%
C=$(42t+27)(49-7t)$\\%
\end{minipage}%
\begin{minipage}{0.5\textwidth}%
D=$(-5-37y)(-21+34y)$\\%
\end{minipage}%
\\%
\begin{minipage}{0.5\textwidth}%
E=$(-47+47z)(-5z+43)$\\%
\end{minipage}%
\begin{minipage}{0.5\textwidth}%
F=$(-3+13t)(-8t+19)$\\%
\end{minipage}%
\\%
\begin{minipage}{0.5\textwidth}%
G=$(9x+31)(50x+26)$\\%
\end{minipage}%
\begin{minipage}{0.5\textwidth}%
H=$(-44t+5)(20+21t)$\\%
\end{minipage}%
\\%
\begin{minipage}{0.5\textwidth}%
I=$(-20z-31)(-28-15z)$\\%
\end{minipage}%
\begin{minipage}{0.5\textwidth}%
J=$(-17z-24)(-44z+33)$\\%
\end{minipage}%
\\%
\begin{minipage}{0.5\textwidth}%
K=$(49-15x)(33x+4)$\\%
\end{minipage}%
\begin{minipage}{0.5\textwidth}%
L=$(-17y-28)(14-23y)$\\%
\end{minipage}%
\\%
\begin{minipage}{0.5\textwidth}%
M=$(9t+29)(-6t-44)$\\%
\end{minipage}%
\begin{minipage}{0.5\textwidth}%
N=$(7t-15)(-50t+12)$\\%
\end{minipage}%
\\%
\begin{minipage}{0.5\textwidth}%
O=$(-29x+31)(27x+1)$\\%
\end{minipage}%
\begin{minipage}{0.5\textwidth}%
P=$(7y-11)(9y-6)$\\%
\end{minipage}%
\\%
\begin{minipage}{0.5\textwidth}%
Q=$(-6t-20)(34-39t)$\\%
\end{minipage}%
\begin{minipage}{0.5\textwidth}%
R=$(16-45y)(-1+17y)$\\%
\end{minipage}%
\\%
\begin{minipage}{0.5\textwidth}%
S=$(45-15y)(34+49y)$\\%
\end{minipage}%
\begin{minipage}{0.5\textwidth}%
T=$(22x+15)(26-49x)$\\%
\end{minipage}%
\\

%
\newpage%
\section{Corrigé}%
\label{sec:Corrig}%
\begin{minipage}{0.5\textwidth}%
A=$(-4y+44)(47-50y)$\\%
A=$-4y \times 47-4y \times (-50y)+44 \times 47+44 \times (-50y)$\\%
A=$-188y+200y^2+2068-2200y$\\%
A=$200y^2-188y-2200y+2068$\\%
A=$200y^2-2388y+2068$\\%
\end{minipage}%
\begin{minipage}{0.5\textwidth}%
B=$(-23+t)(35t+9)$\\%
B=$-23 \times 35t-23 \times 9+t \times 35t+t \times 9$\\%
B=$-805t-207+35t^2+9t$\\%
B=$35t^2-805t+9t-207$\\%
B=$35t^2-796t-207$\\%
\end{minipage}%
\\%
\begin{minipage}{0.5\textwidth}%
C=$(42t+27)(49-7t)$\\%
C=$42t \times 49+42t \times (-7t)+27 \times 49+27 \times (-7t)$\\%
C=$2058t-294t^2+1323-189t$\\%
C=$-294t^2+2058t-189t+1323$\\%
C=$-294t^2+1869t+1323$\\%
\end{minipage}%
\begin{minipage}{0.5\textwidth}%
D=$(-5-37y)(-21+34y)$\\%
D=$-5 \times (-21)-5 \times 34y-37y \times (-21)-37y \times 34y$\\%
D=$105-170y+777y-1258y^2$\\%
D=$-1258y^2-170y+777y+105$\\%
D=$-1258y^2+607y+105$\\%
\end{minipage}%
\\%
\begin{minipage}{0.5\textwidth}%
E=$(-47+47z)(-5z+43)$\\%
E=$-47 \times (-5z)-47 \times 43+47z \times (-5z)+47z \times 43$\\%
E=$235z-2021-235z^2+2021z$\\%
E=$-235z^2+235z+2021z-2021$\\%
E=$-235z^2+2256z-2021$\\%
\end{minipage}%
\begin{minipage}{0.5\textwidth}%
F=$(-3+13t)(-8t+19)$\\%
F=$-3 \times (-8t)-3 \times 19+13t \times (-8t)+13t \times 19$\\%
F=$24t-57-104t^2+247t$\\%
F=$-104t^2+24t+247t-57$\\%
F=$-104t^2+271t-57$\\%
\end{minipage}%
\\%
\begin{minipage}{0.5\textwidth}%
G=$(9x+31)(50x+26)$\\%
G=$9x \times 50x+9x \times 26+31 \times 50x+31 \times 26$\\%
G=$450x^2+234x+1550x+806$\\%
G=$450x^2+1784x+806$\\%
\end{minipage}%
\begin{minipage}{0.5\textwidth}%
H=$(-44t+5)(20+21t)$\\%
H=$-44t \times 20-44t \times 21t+5 \times 20+5 \times 21t$\\%
H=$-880t-924t^2+100+105t$\\%
H=$-924t^2-880t+105t+100$\\%
H=$-924t^2-775t+100$\\%
\end{minipage}%
\\%
\begin{minipage}{0.5\textwidth}%
I=$(-20z-31)(-28-15z)$\\%
I=$-20z \times (-28)-20z \times (-15z)-31 \times (-28)-31 \times (-15z)$\\%
I=$560z+300z^2+868+465z$\\%
I=$300z^2+560z+465z+868$\\%
I=$300z^2+1025z+868$\\%
\end{minipage}%
\begin{minipage}{0.5\textwidth}%
J=$(-17z-24)(-44z+33)$\\%
J=$-17z \times (-44z)-17z \times 33-24 \times (-44z)-24 \times 33$\\%
J=$748z^2-561z+1056z-792$\\%
J=$748z^2+495z-792$\\%
\end{minipage}%
\\%
\begin{minipage}{0.5\textwidth}%
K=$(49-15x)(33x+4)$\\%
K=$49 \times 33x+49 \times 4-15x \times 33x-15x \times 4$\\%
K=$1617x+196-495x^2-60x$\\%
K=$-495x^2+1617x-60x+196$\\%
K=$-495x^2+1557x+196$\\%
\end{minipage}%
\begin{minipage}{0.5\textwidth}%
L=$(-17y-28)(14-23y)$\\%
L=$-17y \times 14-17y \times (-23y)-28 \times 14-28 \times (-23y)$\\%
L=$-238y+391y^2-392+644y$\\%
L=$391y^2-238y+644y-392$\\%
L=$391y^2+406y-392$\\%
\end{minipage}%
\\%
\begin{minipage}{0.5\textwidth}%
M=$(9t+29)(-6t-44)$\\%
M=$9t \times (-6t)+9t \times (-44)+29 \times (-6t)+29 \times (-44)$\\%
M=$-54t^2-396t-174t-1276$\\%
M=$-54t^2-570t-1276$\\%
\end{minipage}%
\begin{minipage}{0.5\textwidth}%
N=$(7t-15)(-50t+12)$\\%
N=$7t \times (-50t)+7t \times 12-15 \times (-50t)-15 \times 12$\\%
N=$-350t^2+84t+750t-180$\\%
N=$-350t^2+834t-180$\\%
\end{minipage}%
\\%
\begin{minipage}{0.5\textwidth}%
O=$(-29x+31)(27x+1)$\\%
O=$-29x \times 27x-29x \times 1+31 \times 27x+31 \times 1$\\%
O=$-783x^2-29x+837x+31$\\%
O=$-783x^2+808x+31$\\%
\end{minipage}%
\begin{minipage}{0.5\textwidth}%
P=$(7y-11)(9y-6)$\\%
P=$7y \times 9y+7y \times (-6)-11 \times 9y-11 \times (-6)$\\%
P=$63y^2-42y-99y+66$\\%
P=$63y^2-141y+66$\\%
\end{minipage}%
\\%
\begin{minipage}{0.5\textwidth}%
Q=$(-6t-20)(34-39t)$\\%
Q=$-6t \times 34-6t \times (-39t)-20 \times 34-20 \times (-39t)$\\%
Q=$-204t+234t^2-680+780t$\\%
Q=$234t^2-204t+780t-680$\\%
Q=$234t^2+576t-680$\\%
\end{minipage}%
\begin{minipage}{0.5\textwidth}%
R=$(16-45y)(-1+17y)$\\%
R=$16 \times (-1)+16 \times 17y-45y \times (-1)-45y \times 17y$\\%
R=$-16+272y+45y-765y^2$\\%
R=$-765y^2+272y+45y-16$\\%
R=$-765y^2+317y-16$\\%
\end{minipage}%
\\%
\begin{minipage}{0.5\textwidth}%
S=$(45-15y)(34+49y)$\\%
S=$45 \times 34+45 \times 49y-15y \times 34-15y \times 49y$\\%
S=$1530+2205y-510y-735y^2$\\%
S=$-735y^2+2205y-510y+1530$\\%
S=$-735y^2+1695y+1530$\\%
\end{minipage}%
\begin{minipage}{0.5\textwidth}%
T=$(22x+15)(26-49x)$\\%
T=$22x \times 26+22x \times (-49x)+15 \times 26+15 \times (-49x)$\\%
T=$572x-1078x^2+390-735x$\\%
T=$-1078x^2+572x-735x+390$\\%
T=$-1078x^2-163x+390$\\%
\end{minipage}%
\\

%
\end{document}